Veritas.Verifier.Global.fsti
@@ -8,19 +8,20 @@ open Veritas.Verifier.Thread
 open FStar.Seq
 open Veritas.SeqAux
 
+module I = Veritas.Interleave
 module MH = Veritas.MultiSetHash
 module V = Veritas.Verifier
 module VT = Veritas.Verifier.Thread
 
 (* Full collection of verifier logs one per thread *)
-let g_vlog = (gl:seq vlog{length gl > 0})
+let g_vlog = seq vlog
 
 let thread_log (gl: g_vlog) (tid: seq_index gl): thread_id_vlog = 
    (tid, index gl tid)
   
 (* globally verifiable logs: every thread-level log is verifiable *)
 let verifiable (gl: g_vlog) = 
-  forall (tid:seq_index gl). {:pattern (thread_log gl tid)} VT.verifiable (thread_log gl tid)
+  forall (tid:seq_index gl). VT.verifiable (thread_log gl tid)
 
 (* Refinement type of logs that are verifiable *)
 let verifiable_log = gl:g_vlog{verifiable gl}
@@ -43,9 +44,3 @@ let hash_verifiable_log = gl:verifiable_log{hash_verifiable gl}
  * in the thread log
  *)
 val clock (gl: verifiable_log) (i: sseq_index gl): timestamp
-
-(* time ordered interleaving of a verifier logs. the "constructor" of the 
- * interleaving contains both the sequence and the proof of the interleaving
- * which helps track the lineage of each entry in the interleaved sequence *)
-val time_seq_ctor (gl: verifiable_log): (interleave_ctor gl)
-
