Veritas.Verifier.TSLog.fsti
@@ -16,147 +16,93 @@ open Veritas.SeqAux
 open FStar.Seq
 
 module E=Veritas.EAC
+module I = Veritas.Interleave
 module V=Veritas.Verifier
 module S = FStar.Seq
 module VT = Veritas.Verifier.Thread
 module VG = Veritas.Verifier.Global
 
+(* an interleaving of vlog_entry *)
+let il_vlog = interleaving vlog_entry
+
+let thread_count (il:il_vlog) = length (I.s_seq il)
+
 (* valid thread id given a number of threads *)
-let valid_tid (p:pos) = tid:nat{tid < p}
+let valid_tid (il:il_vlog) = tid:nat{tid < thread_count il}
 
-(* vlog entry and tid that it went to *)
-let vlog_entry_tid (p:pos) = idx_elem #vlog_entry p
+(* global vlogs that are the source of the interleaving *)
+let g_vlog_of (il: il_vlog): g_vlog =
+  I.s_seq il
 
-(* cast to vlog entry *)
-let to_vlog_entry (#p:pos) (e: vlog_entry_tid p): vlog_entry = 
-  fst e
-
-(* 
- * an indexed sequence log represents and interleaving of a global log (a sequence of thread-level
- * verifier logs. It is a sequence of the form (e,tid) where e denotes a verifier log entry
- * and tid denotes the verifier thread that the entry comes from
- *)
-let idx_seq_vlog (p:pos) = seq (vlog_entry_tid p)
-
-(* 
- * an idx_seq_vlog is verifiable if the global sequence of logs that results from partitioning 
- * by the second element (tid) of a pair is verifiable 
- *)
-let verifiable (#p:pos) (s: idx_seq_vlog p) = 
-  VG.verifiable (partition_idx_seq s)
+(* an interleaving is verifiable if the source logs are verifiable *)
+let verifiable (il: il_vlog) = 
+  VG.verifiable (g_vlog_of il)
 
 (* the clock of an entry in a verifiable idx seq *)
-val clock (#p:pos) (s: idx_seq_vlog p{verifiable s}) (i: seq_index s): timestamp
+val clock (il: il_vlog{verifiable il}) (i: I.seq_index il): timestamp
 
-let clock_sorted (#p:pos) (s: idx_seq_vlog p{verifiable s}) =
-  forall (i:seq_index s). i > 0 ==> clock s (i - 1) `ts_leq` clock s i
+let clock_sorted (il: il_vlog{verifiable il}) =
+  forall (i:I.seq_index il). i > 0 ==> clock il (i - 1) `ts_leq` clock il i
 
-let its_log (p:pos) = 
-  s:idx_seq_vlog p{verifiable s}
+(* TODO: add clock_sorted *)
+let its_log = il:il_vlog{verifiable il}
 
-let hash_verifiable_log (p:pos) = 
-  itsl:its_log p {VG.hash_verifiable (partition_idx_seq itsl)}
+let hash_verifiable_log = 
+  itsl:its_log {VG.hash_verifiable (g_vlog_of itsl)}
 
-val lemma_prefix_verifiable (#p:pos) (itsl: its_log p) (i:nat{i <= length itsl}):
+val lemma_prefix_verifiable (itsl: its_log) (i:nat{i <= I.length itsl}):
   Lemma (requires True)
-        (ensures (verifiable (prefix itsl i)))
-        [SMTPat (prefix itsl i)]
+        (ensures (verifiable (I.prefix itsl i)))
+        [SMTPat (I.prefix itsl i)]
 
 (* create a ts log *)
-val create (gl: VG.verifiable_log): its_log (length gl)
+val create (gl: VG.verifiable_log): (itsl:its_log{g_vlog_of itsl == gl})
 
-(* get back the verifier logs from ts log *)
-let to_g_vlog (#p:pos) (itsl: its_log p): VG.verifiable_log =
-  partition_idx_seq itsl
-
-(* we get back the global logs used to crate ts log with t_g_vlog *)
-val lemma_create_correct (gl: VG.verifiable_log):
-  Lemma (gl = to_g_vlog (create gl))
-
-(* the log entry referenced by the ith entry *)
-let vlog_entry_at (#p:pos) (itsl: its_log p) (i: seq_index itsl): vlog_entry =
-  fst (index itsl i)
-
-(* the key referenced by the i'th entry *)
-let key_of (#p:pos) (e: vlog_entry_tid p): key =
-  V.key_of (to_vlog_entry e)
-
-let key_at (#p:pos) (itsl: its_log p) (i: seq_index itsl): key = 
-  V.key_of (vlog_entry_at itsl i)
-
-let is_add (#p:pos) (e: vlog_entry_tid p): bool = 
-  V.is_add (fst e)
-
-let is_add_of_key (#p:pos) (k:key) (e: vlog_entry_tid p): bool = 
-  is_add e && 
-  key_of e = k
-
-(* is the i'th index of itsl a blum add *)
-let is_blum_add (#p:pos) (ie:vlog_entry_tid p):bool =
-  let (e,_) = ie in
-  match e with
-  | AddB _ _ _ -> true
-  | _ -> false
-
-let is_evict (#p:pos) (e:vlog_entry_tid p): bool = 
-  V.is_evict (to_vlog_entry e)
-
-(* is the index i of ts log an blum evict *)
-let is_blum_evict (#p:pos) (ie:vlog_entry_tid p): bool = 
-  let (e,_) = ie in
-  match e with
-  | EvictB _ _ -> true
-  | EvictBM _ _ _ -> true
-  | _ -> false
-
-let is_evict_of_key (k:key) (#p:pos) (ie:vlog_entry_tid p): bool = 
-  is_evict ie &&
-  key_of ie = k
+let key_at (itsl: its_log) (i: I.seq_index itsl): key = 
+  V.key_of (I.index itsl i)
   
-let has_next_add_of_key (#p:pos) (itsl: its_log p) (i:seq_index itsl) (k:key): bool =
-  has_next (is_add_of_key k) itsl i
+let has_next_add_of_key (itsl: its_log) (i: I.seq_index itsl) (k:key): bool =
+  has_next (is_add_of_key k) (I.i_seq itsl) i
 
-let next_add_of_key (#p:pos) 
-  (itsl: its_log p) 
-  (i:seq_index itsl) (k:key{has_next_add_of_key itsl i k}): 
-  (j:seq_index itsl{j > i && is_add_of_key k (index itsl j)}) = 
-  next_index (is_add_of_key k) itsl i
+let next_add_of_key
+  (itsl: its_log) 
+  (i:I.seq_index itsl) 
+  (k:key{has_next_add_of_key itsl i k}): 
+  (j:I.seq_index itsl{j > i && is_add_of_key k (I.index itsl j)}) = 
+  next_index (is_add_of_key k) (I.i_seq itsl) i
 
-let is_entry_of_key (k:key) (#p:pos) (e:vlog_entry_tid p): bool = 
+let is_entry_of_key (k:key) (e:vlog_entry): bool = 
   key_of e = k
 
-let has_some_entry_of_key (#p:pos) (itsl: its_log p) (k:key): bool = 
-  exists_sat_elems (is_entry_of_key k) itsl
+let has_some_entry_of_key (itsl: its_log) (k:key): bool = 
+  exists_sat_elems (is_entry_of_key k) (I.i_seq itsl)
 
-let last_idx_of_key (#p:pos) (itsl: its_log p) (k:key{has_some_entry_of_key itsl k}):
-  seq_index itsl = 
-  last_index (is_entry_of_key k) itsl
-
-let add_method_of (#p:pos) (e:vlog_entry_tid p{is_add e}): add_method = 
-  V.addm_of_entry (to_vlog_entry e)
+let last_idx_of_key (itsl: its_log) (k:key{has_some_entry_of_key itsl k}):
+  I.seq_index itsl = 
+  last_index (is_entry_of_key k) (I.i_seq itsl)
 
 (* does the key k have some add *)
-let has_some_add_of_key (#p:pos) (itsl: its_log p) (k:key): bool = 
-  exists_sat_elems (is_add_of_key k) itsl
+let has_some_add_of_key (itsl: its_log) (k:key): bool = 
+  exists_sat_elems (is_add_of_key k) (I.i_seq itsl)
 
-(* when the eac state of a key is instore return the index of the last add that transitioned
- * the key k to "instore" *)
-val last_add_idx (#p:pos) (itsl: its_log p) (k: key{has_some_add_of_key itsl k}): 
-  (i:seq_index itsl{is_add_of_key k (index itsl i)})
+(* the last add index of a key *)
+let last_add_idx (itsl: its_log) (k: key{has_some_add_of_key itsl k}): 
+  (i:I.seq_index itsl{is_add_of_key k (I.index itsl i)}) = 
+  last_index (is_add_of_key k) (I.i_seq itsl)
 
 (* thread id of the ith entry *)
-let thread_id_of (#p:pos) (itsl: its_log p) (i: seq_index itsl): valid_tid p =
-  snd (index itsl i)  
+let thread_id_of (itsl: its_log) (i: I.seq_index itsl): valid_tid itsl =
+  fst (i2s_map itsl i)
 
 (* the verifier thread where the last add of key k happens *)
-let last_add_tid (#p:pos) (itsl: its_log p) (k: key{has_some_add_of_key itsl k}): valid_tid p =
+let last_add_tid (itsl: its_log) (k: key{has_some_add_of_key itsl k}): valid_tid itsl =
   thread_id_of itsl (last_add_idx itsl k)
 
 (*thread state after processing ts log - guaranteed to be valid *)
-val thread_state (#p:pos) (itsl: its_log p) (tid: valid_tid p): (vs:vtls{Valid? vs})
+val thread_state (itsl: its_log) (tid: valid_tid itsl): (vs:vtls{Valid? vs})
 
 (* thread store after processing ts log *)
-let thread_store (#p:pos) (itsl: its_log p) (tid: valid_tid p): vstore =
+let thread_store (itsl: its_log) (tid: valid_tid itsl): vstore =
   Valid?.st (thread_state itsl tid)
 
 (* 
@@ -164,102 +110,102 @@ let thread_store (#p:pos) (itsl: its_log p) (tid: valid_tid p): vstore =
  * this lemma states that state of tid at (i+1) is obtained by the state at (i) 
  * applying the vlog entry at i.
  *)
-val lemma_verifier_thread_state_extend (#p:pos) (itsl: its_log p) (i:seq_index itsl):
-  Lemma (thread_state (prefix itsl (i + 1)) (thread_id_of itsl i)== 
-         t_verify_step (thread_state (prefix itsl i) (thread_id_of itsl i))
-                       (vlog_entry_at itsl i))
+val lemma_verifier_thread_state_extend (itsl: its_log) (i: I.seq_index itsl):
+  Lemma (thread_state (I.prefix itsl (i + 1)) (thread_id_of itsl i) == 
+         t_verify_step (thread_state (I.prefix itsl i) (thread_id_of itsl i))
+                       (I.index itsl i))
 
 (* is this an evict add consistent log *)
-val is_eac (#p:pos) (itsl: its_log p):bool
+val is_eac (itsl: its_log):bool
 
 (* eac ts log *)
-let eac_log (p:pos) = itsl: its_log p {is_eac itsl}
+let eac_log = itsl: its_log {is_eac itsl}
 
 (* non-eac ts log *)
-type neac_log (p:pos) = itsl: its_log p {not (is_eac itsl)}
+type neac_log = itsl: its_log {not (is_eac itsl)}
 
 (* if itsl is eac, then any prefix is also eac *)
-val lemma_eac_implies_prefix_eac (#p:pos) (itsl: eac_log p) (i:nat {i <= length itsl}):
+val lemma_eac_implies_prefix_eac (itsl: eac_log) (i:nat {i <= I.length itsl}):
   Lemma (requires True)
-        (ensures (is_eac (prefix itsl i)))
-        [SMTPat (prefix itsl i)]
+        (ensures (is_eac (I.prefix itsl i)))
+        [SMTPat (I.prefix itsl i)]
 
 (* the eac state of a key at the end of an its log *)
-val eac_state_of_key (#p:pos) (itsl: its_log p) (k:key): eac_state 
+val eac_state_of_key (itsl: its_log) (k:key): eac_state 
 
 (* by definition, ts log is eac_valid only if the state of each key is not EACFail *)
-val lemma_eac_state_of_key_valid (#p:pos) (itsl: eac_log p) (k:key):
+val lemma_eac_state_of_key_valid (itsl: eac_log) (k:key):
   Lemma (EACFail <> eac_state_of_key itsl k)
 
 (* is the eac state of key at the end of its_log init *)
-let is_eac_state_init (#p:pos) (itsl: its_log p) (k:key): bool =
+let is_eac_state_init (itsl: its_log) (k:key): bool =
   eac_state_of_key itsl k = EACInit
 
 (* is the key k in evicted state in *)
-let is_eac_state_evicted (#p:pos) (itsl: its_log p) (k:key): bool = 
+let is_eac_state_evicted (itsl: its_log) (k:key): bool = 
   EACEvictedMerkle? (eac_state_of_key itsl k) ||
   EACEvictedBlum? (eac_state_of_key itsl k) 
 
-let eac_state_evicted_value (#p:pos) (itsl: its_log p) (k:key{is_eac_state_evicted itsl k}): value =
+let eac_state_evicted_value (itsl: its_log) (k:key{is_eac_state_evicted itsl k}): value =
   let st = eac_state_of_key itsl k in
   match st with
   | EACEvictedMerkle v -> v
   | EACEvictedBlum v _ _ -> v
 
 (* is the key currently evicted into merkle *)
-let is_eac_state_evicted_merkle (#p:pos) (itsl: its_log p) (k:key): bool = 
+let is_eac_state_evicted_merkle (itsl: its_log) (k:key): bool = 
   let st = eac_state_of_key itsl k in
   match st with
   | EACEvictedMerkle v -> true
   | _ -> false
 
 (* is the key currently evicted into merkle *)
-let is_eac_state_evicted_blum (#p:pos) (itsl: its_log p) (k:key): bool = 
+let is_eac_state_evicted_blum (itsl: its_log) (k:key): bool = 
   let st = eac_state_of_key itsl k in
   match st with
   | EACEvictedBlum v t j -> true
   | _ -> false
 
 (* is the key k in instore state after processing its_log *)
-let is_eac_state_instore (#p:pos) (itsl: its_log p) (k:key):bool = 
+let is_eac_state_instore (itsl: its_log) (k:key):bool = 
   EACInStore? (eac_state_of_key itsl k)
 
-let is_eac_state_active (#p:pos) (itsl: its_log p) (k:key): bool = 
+let is_eac_state_active (itsl: its_log) (k:key): bool = 
   is_eac_state_evicted itsl k ||
   is_eac_state_instore itsl k
 
 (* the extended vlog entry to use for eac checking *)
-val vlog_entry_ext_at (#p:pos) (itsl: its_log p) (i:seq_index itsl): 
-  (e:vlog_entry_ext{E.to_vlog_entry e = vlog_entry_at itsl i})
+val vlog_entry_ext_at (itsl: its_log) (i:I.seq_index itsl): 
+  (e:vlog_entry_ext{E.to_vlog_entry e = I.index itsl i})
 
 (* the eac state transition induced by the i'th entry *)
-val lemma_eac_state_transition (#p:pos) (itsl: its_log p) (i:seq_index itsl):
-  Lemma (eac_state_of_key (prefix itsl (i + 1)) (key_at itsl i) = 
+val lemma_eac_state_transition (itsl: its_log) (i:I.seq_index itsl):
+  Lemma (eac_state_of_key (I.prefix itsl (i + 1)) (key_at itsl i) = 
          eac_add (vlog_entry_ext_at itsl i) 
-                 (eac_state_of_key (prefix itsl i) (key_at itsl i)))
+                 (eac_state_of_key (I.prefix itsl i) (key_at itsl i)))
 
 (* when the eac state of a key is "instore" then there is always a previous add *)
-val lemma_eac_state_active_implies_prev_add (#p:pos) (itsl: eac_log p) 
+val lemma_eac_state_active_implies_prev_add (itsl: eac_log) 
   (k:key{is_eac_state_active itsl k}):
   Lemma (requires True)
         (ensures (has_some_add_of_key itsl k))
         [SMTPat (is_eac_state_instore itsl k)]
 
 (* add method of an eac state *)
-val lemma_eac_state_addm (#p:pos) (itsl: eac_log p) (k:key{is_eac_state_instore itsl k}):
+val lemma_eac_state_addm (itsl: eac_log) (k:key{is_eac_state_instore itsl k}):
   Lemma (E.add_method_of (eac_state_of_key itsl k) = 
-         add_method_of (index itsl (last_add_idx itsl k)))
+         V.addm_of_entry (I.index itsl (last_add_idx itsl k)))
 
 (* the evicted value is always of the correct type for the associated key *)
-val lemma_eac_value_correct_type (#p:pos) (itsl: eac_log p) (k:key):  
+val lemma_eac_value_correct_type (itsl: eac_log) (k:key):  
   Lemma (requires (E.is_eac_state_active (eac_state_of_key itsl k)))
         (ensures is_value_of k (E.value_of (eac_state_of_key itsl k)))
 
 (* value associated with eac state *)
-val eac_state_value (#n:pos) (itsl: eac_log n) (k:key{is_eac_state_active itsl k}): value_type_of k
+val eac_state_value (itsl: eac_log) (k:key{is_eac_state_active itsl k}): value_type_of k
 
 (* we never see operations on Root so its eac state is always init *)
-val lemma_eac_state_of_root_init (#p:pos) (itsl: eac_log p):
+val lemma_eac_state_of_root_init (itsl: eac_log):
   Lemma (is_eac_state_init itsl Root)
 
 (* 
@@ -267,67 +213,67 @@ val lemma_eac_state_of_root_init (#p:pos) (itsl: eac_log p):
  * thread contains the key in its store. Valid only for non-root keys 
  * since we start off with the root in the cache of thread 0
  *)
-val lemma_eac_state_init_store (#p:pos) (itsl: eac_log p) (k: key) (tid:valid_tid p):
+val lemma_eac_state_init_store (itsl: eac_log) (k: key) (tid:valid_tid itsl):
   Lemma (requires (k <> Root && is_eac_state_init itsl k))
         (ensures (not (store_contains (thread_store itsl tid) k)))
 
 (* when the eac state of a key is evicted then no thread contains the key in its store *)
-val lemma_eac_state_evicted_store  (#p:pos) (itsl: eac_log p) (k: key{is_eac_state_evicted itsl k}) 
-  (tid:valid_tid p):
+val lemma_eac_state_evicted_store  (itsl: eac_log) (k: key{is_eac_state_evicted itsl k}) 
+  (tid:valid_tid itsl):
   Lemma (not (store_contains (thread_store itsl tid) k))
 
 (* when the eac_state of k is instore, then k is in the store of a unique verifier thread *)
-val stored_tid (#p:pos) (itsl: eac_log p) (k:key{is_eac_state_instore itsl k}): 
-  (tid: valid_tid p{store_contains (thread_store itsl tid) k})
+val stored_tid (itsl: eac_log) (k:key{is_eac_state_instore itsl k}): 
+  (tid: valid_tid itsl{store_contains (thread_store itsl tid) k})
 
 (* uniqueness: k is not in any store other than stored_tid *)
-val lemma_key_in_unique_store (#p:pos) (itsl: eac_log p) (k:key) (tid: valid_tid p):
+val lemma_key_in_unique_store (itsl: eac_log) (k:key) (tid: valid_tid itsl):
   Lemma (requires (is_eac_state_instore itsl k /\ tid <> stored_tid itsl k))
         (ensures (not (store_contains (thread_store itsl tid) k)))
 
 (* it is therefore meaningful to talk of the stored value of a key *)
-let stored_value (#p:pos) (itsl: eac_log p) (k:key{is_eac_state_instore itsl k}): value_type_of k =
+let stored_value (itsl: eac_log) (k:key{is_eac_state_instore itsl k}): value_type_of k =
   V.stored_value (thread_store itsl (stored_tid itsl k)) k
 
-let stored_add_method (#p:pos) (itsl: eac_log p) (k:key {is_eac_state_instore itsl k}): add_method =
+let stored_add_method (itsl: eac_log) (k:key {is_eac_state_instore itsl k}): add_method =
   V.add_method_of (thread_store itsl (stored_tid itsl k)) k
 
 (* for data keys, the value in the store is the same as the value associated with the eac state *)
-val lemma_eac_stored_value (#p:pos) (itsl: eac_log p) (k: data_key{is_eac_state_instore itsl k}):
+val lemma_eac_stored_value (itsl: eac_log) (k: data_key{is_eac_state_instore itsl k}):
   Lemma (eac_state_value itsl k = stored_value itsl k)
 
 (* 
  * for all keys, the add method stored in the store is the same as the add method associated 
  * with eac state
  *)
-val lemma_eac_stored_addm (#p:pos) (itsl: eac_log p) (k:key{is_eac_state_instore itsl k}):
+val lemma_eac_stored_addm (itsl: eac_log) (k:key{is_eac_state_instore itsl k}):
   Lemma (E.add_method_of (eac_state_of_key itsl k) = stored_add_method itsl k)
   
 (* if k is in a verifier store, then its eac_state is instore *)
-val lemma_instore_implies_eac_state_instore (#p:pos) (itsl:eac_log p) (k:key{k <> Root}) (tid:valid_tid p):
+val lemma_instore_implies_eac_state_instore (itsl:eac_log) (k:key{k <> Root}) (tid:valid_tid itsl):
   Lemma (store_contains (thread_store itsl tid) k ==> is_eac_state_instore itsl k)
          
 (* the root is always in thread 0 *)
-val lemma_root_in_store0 (#p:pos) (itsl: eac_log p):
+val lemma_root_in_store0 (itsl: eac_log{thread_count itsl > 0}):
   Lemma (store_contains (thread_store itsl 0) Root)
 
-val lemma_root_not_in_store (#p:pos) (itsl: eac_log p) (tid:valid_tid p):
+val lemma_root_not_in_store (itsl: eac_log) (tid:valid_tid itsl{tid > 0}):
   Lemma (not (store_contains (thread_store itsl tid) Root))
 
 (* we use eac constraints to associate a value with each key *)
-val eac_value (#p:pos) (itsl: eac_log p) (k:key): value_type_of k
+val eac_value (itsl: eac_log) (k:key): value_type_of k
 
 (* eac_value is consistent with stored value *)
-val lemma_eac_value_is_stored_value (#p:pos) (itsl: eac_log p) (k:key) (tid: valid_tid p):  
+val lemma_eac_value_is_stored_value (itsl: eac_log) (k:key) (tid: valid_tid itsl):  
   Lemma (requires (store_contains (thread_store itsl tid) k))
         (ensures (eac_value itsl k = V.stored_value (thread_store itsl tid) k))
 
-val lemma_eac_value_is_evicted_value (#p:pos) (itsl: eac_log p) (k:key):
+val lemma_eac_value_is_evicted_value (itsl: eac_log) (k:key):
   Lemma (requires (is_eac_state_evicted itsl k))
         (ensures (eac_state_evicted_value itsl k = eac_state_value itsl k))
 
-val lemma_ext_evict_val_is_stored_val (#p:pos) (itsl: its_log p) (i: seq_index itsl):
-  Lemma (requires (is_evict (index itsl i)))
+val lemma_ext_evict_val_is_stored_val (itsl: its_log) (i: I.seq_index itsl):
+  Lemma (requires (is_evict (I.index itsl i)))
         (ensures (store_contains (thread_store itsl (thread_id_of itsl i)) (key_at itsl i) /\
                   is_evict_ext (vlog_entry_ext_at itsl i) /\
                   V.stored_value (thread_store itsl (thread_id_of itsl i)) (key_at itsl i) = 
@@ -335,10 +281,8 @@ val lemma_ext_evict_val_is_stored_val (#p:pos) (itsl: its_log p) (i: seq_index i
 
 (* if an evict is not the last entry of a key, then there is a add subsequent to the 
  * evict *)
-val lemma_evict_has_next_add (#p:pos) (itsl: its_log p) (i:seq_index itsl):
-  Lemma (requires (is_evict (index itsl i) /\
-                   exists_sat_elems (is_entry_of_key (key_of (index itsl i))) itsl) /\
-                   i < last_idx_of_key itsl (key_of (index itsl i)))
-        (ensures (has_next_add_of_key itsl i (key_of (index itsl i))))
-
-                  
+val lemma_evict_has_next_add (itsl: its_log) (i:I.seq_index itsl):
+  Lemma (requires (is_evict (I.index itsl i) /\
+                   exists_sat_elems (is_entry_of_key (key_of (I.index itsl i))) (I.i_seq itsl)) /\
+                   i < last_idx_of_key itsl (key_of (I.index itsl i)))
+        (ensures (has_next_add_of_key itsl i (key_of (I.index itsl i))))
